theories/lang/lang_extra.v
@@ -6,105 +6,97 @@ From stdpp Require Import list.
 
 Section lang_extra.
 
-Context `{HyperConst : !HypervisorConstants}.
-Context `{HyperParams : !HypervisorParameters}.
+  Context `{HyperConst : !HypervisorConstants}.
+  Context `{HyperParams : !HypervisorParameters}.
 
-Implicit Type σ : state.
+  Implicit Type σ : state.
 
-Lemma check_access_page_mem_eq {σ i a} :
-  check_access_page σ i (to_pid_aligned a) =
-  check_access_addr σ i a.
-Proof.
-  rewrite /check_access_addr; done.
-Qed.
-
-Lemma list_pid_to_addr_NoDup (ps:list PID):
-  NoDup ps ->
-  NoDup (list_pid_to_addr ps).
-Proof.
-  intro Hnd.
-  rewrite /list_pid_to_addr.
-  induction ps.
-  - simpl. by apply NoDup_nil.
-  - cbn.  apply  NoDup_app.
-    split.
-    { apply finz_seq_NoDup'. apply last_addr_in_bound. }
-    split.
-    { intros. apply NoDup_cons in Hnd. destruct Hnd as [ Hnotin Hnd].
-      pose proof (finz_seq_in2 _ _ _ H) as Halt.
-      pose proof (finz_seq_in1 _ _ _ H) as Hagt.
-      clear IHps.
-      induction ps.
-      cbn.
-      apply not_elem_of_nil.
-      cbn.
-      apply not_elem_of_app.
+  Lemma list_pid_to_addr_NoDup (ps:list PID):
+    NoDup ps ->
+    NoDup (list_pid_to_addr ps).
+  Proof.
+    intro Hnd.
+    rewrite /list_pid_to_addr.
+    induction ps.
+    - simpl. by apply NoDup_nil.
+    - cbn.  apply  NoDup_app.
       split.
-      { intro.
-        pose proof (finz_seq_in2 _ _ _ H0) as Ha0lt.
-        pose proof (finz_seq_in1 _ _ _ H0) as Ha0gt.
-        assert (Hne: a ≠ a0).
-        apply not_elem_of_cons in Hnotin.
-        destruct Hnotin;eauto.
-        destruct (decide ((of_pid a)<= (of_pid a0))%f).
-        assert (Hlt: ((of_pid a)< (of_pid a0))%f).
-        assert (Hne': ((of_pid a) ≠ (of_pid a0))%f).
-        intro.
-        apply Hne.
-        apply of_pid_eq;eauto.
-        solve_finz.
-        clear l Hne.
-        assert ((a ^+ (Z.of_nat (Z.to_nat page_size) - 1)) < a0 )%f.
-        apply pid_lt_lt;eauto.
-        solve_finz.
-        assert (a0<a)%f.
-        solve_finz.
-        assert ((a0 ^+ (Z.of_nat (Z.to_nat page_size) - 1)) < a )%f.
-        apply pid_lt_lt;eauto.
-        solve_finz.
+      { apply finz_seq_NoDup'. apply last_addr_in_bound. }
+      split.
+      { intros. apply NoDup_cons in Hnd. destruct Hnd as [ Hnotin Hnd].
+        pose proof (finz_seq_in2 _ _ _ H) as Halt.
+        pose proof (finz_seq_in1 _ _ _ H) as Hagt.
+        clear IHps.
+        induction ps.
+        cbn.
+        apply not_elem_of_nil.
+        cbn.
+        apply not_elem_of_app.
+        split.
+        { intro.
+          pose proof (finz_seq_in2 _ _ _ H0) as Ha0lt.
+          pose proof (finz_seq_in1 _ _ _ H0) as Ha0gt.
+          assert (Hne: a ≠ a0).
+          apply not_elem_of_cons in Hnotin.
+          destruct Hnotin;eauto.
+          destruct (decide ((of_pid a)<= (of_pid a0))%f).
+          assert (Hlt: ((of_pid a)< (of_pid a0))%f).
+          assert (Hne': ((of_pid a) ≠ (of_pid a0))%f).
+          intro.
+          apply Hne.
+          apply of_pid_eq;eauto.
+          solve_finz.
+          clear l Hne.
+          assert ((a ^+ (Z.of_nat (Z.to_nat page_size) - 1)) < a0 )%f.
+          apply pid_lt_lt;eauto.
+          solve_finz.
+          assert (a0<a)%f.
+          solve_finz.
+          assert ((a0 ^+ (Z.of_nat (Z.to_nat page_size) - 1)) < a )%f.
+          apply pid_lt_lt;eauto.
+          solve_finz.
+        }
+        apply IHps.
+        { apply not_elem_of_cons in Hnotin;destruct Hnotin;done. }
+        { apply NoDup_cons in Hnd;destruct Hnd;done. }
       }
       apply IHps.
-      { apply not_elem_of_cons in Hnotin;destruct Hnotin;done. }
-      { apply NoDup_cons in Hnd;destruct Hnd;done. }
+      apply NoDup_cons in Hnd;destruct Hnd;done.
+  Qed.
+
+  Lemma flat_list_list_word_length_eq wss wss':
+    length wss = length wss'->
+    (forall ws, ws ∈ wss -> length ws = (Z.to_nat page_size)) ->
+    (forall ws', ws' ∈ wss' -> length ws' = (Z.to_nat page_size)) ->
+    length (flat_list_list_word wss) = length (flat_list_list_word wss').
+  Proof.
+    intro Heqlen.
+    rewrite /flat_list_list_word.
+    generalize dependent wss'.
+    induction wss;destruct wss';cbn;
+      intros Heqlen' Hws Hws'; try inversion Heqle;eauto.
+    inversion Heqlen'.
+    inversion Heqlen'.
+    rewrite !app_length.
+    rewrite (IHwss wss');eauto.
+    2:{
+      intros ws Hin.
+      apply Hws.
+      apply elem_of_cons;right;done.
     }
-    apply IHps.
-    apply NoDup_cons in Hnd;destruct Hnd;done.
-Qed.
+    2:{
+      intros ws' Hin.
+      apply Hws'.
+      apply elem_of_cons;right;done.
+    }
+    f_equal.
+    rewrite (Hws a).
+    rewrite (Hws' l) //.
+    apply elem_of_cons;left;done.
+    apply elem_of_cons;left;done.
+  Qed.
 
-Lemma flat_list_list_word_length_eq wss wss':
-  length wss = length wss'->
-  (forall ws, ws ∈ wss -> length ws = (Z.to_nat page_size)) ->
-  (forall ws', ws' ∈ wss' -> length ws' = (Z.to_nat page_size)) ->
-  length (flat_list_list_word wss) = length (flat_list_list_word wss').
-Proof.
-  intro Heqlen.
-  rewrite /flat_list_list_word.
-  generalize dependent wss'.
-  induction wss;destruct wss';cbn;
-  intros Heqlen' Hws Hws'; try inversion Heqle;eauto.
-  inversion Heqlen'.
-  inversion Heqlen'.
-  rewrite !app_length.
-  rewrite (IHwss wss');eauto.
-  2:{
-    intros ws Hin.
-    apply Hws.
-    apply elem_of_cons;right;done.
-  }
-  2:{
-    intros ws' Hin.
-    apply Hws'.
-    apply elem_of_cons;right;done.
-  }
-  f_equal.
-  rewrite (Hws a).
-  rewrite (Hws' l) //.
-  apply elem_of_cons;left;done.
-  apply elem_of_cons;left;done.
-Qed.
-
-
-(* lemmas about transactions *)
+(** lemmas about transactions *)
 
   Definition serialized_memory_descirptor l (r:VMID) ps := [l; (of_imm (encode_vmid r))]++ (map (λ pid, (of_pid pid)) ps).
 
@@ -124,12 +116,11 @@ Qed.
   Qed.
 
   Lemma mem_desc_valid{ b psd σ} l (ps : list PID):
-   l =  (length ps) ->
-   psd =  (map (λ pid, (of_pid pid)) ps) ->
+   l = (length ps) ->
+   psd = (map (λ pid, (of_pid pid)) ps) ->
    (∀ (k : nat) (y1 y2 : Addr),
             finz.seq b (length psd) !! k = Some y1 → psd !! k = Some y2 → get_mem σ !! y1 = Some y2) ->
-   map (λ v : Addr,(bind ((get_mem σ) !! v) to_pid )) (finz.seq b l)
-   = map (λ pid, Some pid) ps.
+   map (λ v : Addr,(bind ((get_mem σ) !! v) to_pid )) (finz.seq b l) = map (λ pid, Some pid) ps.
   Proof.
     intros.
     generalize dependent b.
@@ -176,25 +167,25 @@ Qed.
   Qed.
 
   Lemma sequence_a_map_unit{A} (l:list A) :
-  @sequence_a list _ _ _ A option _ _ (map (λ e , Some e ) l) = Some l.
-    Proof.
-      unfold sequence_a.
-      simpl.
-      unfold monad.List.sequence_a_list.
-      induction l.
-      done.
-      simpl.
-      simpl in IHl.
-      rewrite IHl //.
-Qed.
+    @sequence_a list _ _ _ A option _ _ (map (λ e , Some e ) l) = Some l.
+  Proof.
+    unfold sequence_a.
+    simpl.
+    unfold monad.List.sequence_a_list.
+    induction l.
+    done.
+    simpl.
+    simpl in IHl.
+    rewrite IHl //.
+  Qed.
 
   Lemma transaction_descriptor_valid{i j wf l psd σ} des p :
     (finz.to_z l) = (Z.of_nat (length psd)) ->
     des = serialized_transaction_descriptor i j wf l psd W0 ->
     seq_in_page (of_pid p) (length des) p ->
     (∀ (k : nat) (y1 y2 : Addr),
-             finz.seq (of_pid p) (length des) !! k = Some y1 → des !! k = Some y2 → get_mem σ !! y1 = Some y2) ->
-   parse_transaction_descriptor σ p = Some (i , None, wf,  j , list_to_set psd).
+       finz.seq (of_pid p) (length des) !! k = Some y1 → des !! k = Some y2 → get_mem σ !! y1 = Some y2) ->
+    parse_transaction_descriptor σ p = Some (i , None, wf,  j , list_to_set psd).
   Proof.
     intros.
     rewrite /parse_transaction_descriptor /get_memory_with_offset.
@@ -292,55 +283,62 @@ Qed.
   Qed.
 
 
-  (* lemmas about taking a step *)
-
+  (** lemmas about taking a step *)
 
   Lemma reducible_normal{σ} i instr ai wi :
    (get_current_vm σ) = i ->
-   check_access_addr σ i ai = true ->
+   check_access_page σ i (tpa ai) = true ->
+   (get_mail_box σ @ i).1 ≠ (tpa ai) ->
    get_reg σ PC = Some ai ->
    get_mem σ !! ai = Some wi ->
    decode_instruction wi = Some (instr) ->
    ∃ m' σ', step ExecI σ m' σ'.
   Proof.
-    intros.
+    intros Hi Hcheck Hneq Hpc Hai Hdecode.
     remember (exec instr σ) as ex.
     exists ex.1 ,ex.2 .
     apply step_exec_normal with ai wi instr;subst i ;eauto.
-    + by rewrite /is_valid_PC H1 /= H0.
-    + by rewrite /get_memory H0.
+    rewrite /read_memory /check_read_access_addr /check_read_access_page.
+    rewrite Hcheck.
+    rewrite andb_true_l.
+    case_match.
+    done.
+    apply bool_decide_eq_false in Heqb.
+    done.
    Qed.
 
   Lemma step_ExecI_normal {σ m' σ' } i instr ai wi  :
    step ExecI σ m' σ'->
    (get_current_vm σ) = i ->
-   check_access_addr σ i ai = true ->
+   check_access_page σ i (tpa ai) = true ->
+   (get_mail_box σ @ i).1 ≠ (tpa ai) ->
    get_reg σ PC = Some ai ->
    get_mem σ !! ai = Some wi ->
    decode_instruction wi = Some (instr) ->
    (exec instr σ).1 = m' ∧ (exec instr σ).2 = σ'.
   Proof.
-    intros HstepP Heqi Hacc HPC Hmem Hdecode.
+    intros HstepP Heqi Hcheck Hneq HPC Hmem Hdecode.
     inversion HstepP as
-        [ σ1' Hinvalid
-        | σ1' Ha w _ Hdecode' Hmem' Hinvalid_ins
-        | σ1'  ? ? ? ? Hvalid Hreg2 Hmem2 Hdecode2 Hexec Hcontrol];
+        [ σ1' a Hcheck' Hread
+        | σ1' a w Hpc' Hread Hdecode' Hinvalid_ins
+        | σ1'  ? ? ? ? Hreg2 Hread Hdecode2 Hexec Hcontrol];
       simplify_eq /=.
-    + (*Fail*)
-      by rewrite /is_valid_PC //= HPC Hacc in Hinvalid.
-    + rewrite /get_memory Hacc Hmem in Hmem'.
-      inversion Hmem';subst.
-      rewrite Hdecode // in Hinvalid_ins.
-    + (* Normal. *)
-      (* eliminate Hmem2 *)
-      rewrite /get_memory  Hacc Hmem in Hmem2 .
-      inversion Hmem2;subst wi; clear Hmem2.
-      (* eliminate Hdecode2 *)
+    + rewrite /read_memory Hmem /check_read_access_addr /check_read_access_page Hcheck andb_true_l /= in Hread.
+      case_bool_decide;done.
+    + rewrite /read_memory /check_read_access_addr /check_read_access_page Hcheck andb_true_l /= in Hread.
+      case_bool_decide;last done.
+      rewrite Hread in Hmem.
+      inversion Hmem;subst.
+      rewrite Hdecode // in Hdecode'.
+    + rewrite /read_memory /check_read_access_addr /check_read_access_page Hcheck andb_true_l /= in Hread.
+      case_bool_decide;last done.
+      rewrite Hread in Hmem.
+      inversion Hmem;subst.
       by rewrite Hdecode in Hdecode2;inversion Hdecode2;subst i0.
   Qed.
 
- Lemma option_state_unpack_preserve_state_Some σ1 σ2 (σ2': option state) :
-   σ2' = Some σ2 ->  (ExecI, σ2) = (option_state_unpack σ1 σ2').
+  Lemma option_state_unpack_preserve_state_Some σ1 σ2 (σ2': option state) :
+    σ2' = Some σ2 -> (ExecI, σ2) = (option_state_unpack σ1 σ2').
   Proof.
     intros.
     destruct σ2' eqn:Heqn.
@@ -350,21 +348,22 @@ Qed.
   Qed.
 
   Lemma mov_word_ExecI σ1 r w :
-   PC ≠ r -> NZ ≠ r -> (mov_word σ1 r w)= (ExecI, (update_incr_PC (update_reg σ1 r w))).
+    PC ≠ r -> NZ ≠ r ->
+    (mov_word σ1 r w) = (ExecI, (update_incr_PC (update_reg σ1 r w))).
   Proof.
     intros.
     unfold mov_word .
     destruct r;[contradiction|contradiction|].
     rewrite <- (option_state_unpack_preserve_state_Some
-                 σ1 (update_incr_PC (update_reg σ1 (R n fin) w))
-                 (Some (update_incr_PC (update_reg σ1 (R n fin) w))));eauto.
+                  σ1 (update_incr_PC (update_reg σ1 (R n fin) w))
+                  (Some (update_incr_PC (update_reg σ1 (R n fin) w))));eauto.
   Qed.
 
   Lemma mov_reg_ExecI σ1 r1 r2 w:
-   PC ≠ r1 -> NZ ≠ r1 ->
-   PC ≠ r2 -> NZ ≠ r2 ->
-   (get_reg σ1 r2) = Some w ->
-   (mov_reg σ1 r1 r2)= (ExecI, (update_incr_PC (update_reg σ1 r1 w))).
+    PC ≠ r1 -> NZ ≠ r1 ->
+    PC ≠ r2 -> NZ ≠ r2 ->
+    (get_reg σ1 r2) = Some w ->
+    (mov_reg σ1 r1 r2) = (ExecI, (update_incr_PC (update_reg σ1 r1 w))).
   Proof.
     intros.
     unfold mov_reg.
@@ -373,140 +372,121 @@ Qed.
     simpl.
     rewrite H3.
     rewrite <- (option_state_unpack_preserve_state_Some
-                 σ1 (update_incr_PC (update_reg σ1 (R n fin) w))
-                 (Some (update_incr_PC (update_reg σ1 (R n fin) w))));eauto.
+                  σ1 (update_incr_PC (update_reg σ1 (R n fin) w))
+                  (Some (update_incr_PC (update_reg σ1 (R n fin) w))));eauto.
   Qed.
 
-  Lemma ldr_ExecI σ1 r1 r2 a w:
-   PC ≠ r1 -> NZ ≠ r1 ->
-   PC ≠ r2 -> NZ ≠ r2 ->
-   (get_mail_boxes σ1 !!! get_current_vm σ1).1 ≠ (to_pid_aligned a) ->
-   (get_reg σ1 r2) = Some a ->
-   get_memory σ1 a = Some w ->
-   (ldr σ1 r1 r2)= (ExecI, (update_incr_PC (update_reg σ1 r1 w))).
+  Lemma ldr_ExecI σ r1 r2 a w:
+    PC ≠ r1 -> NZ ≠ r1 ->
+    PC ≠ r2 -> NZ ≠ r2 ->
+    (get_mail_box σ @ (get_current_vm σ)).1 ≠ (tpa a) ->
+    check_access_page σ (get_current_vm σ) (tpa a) = true ->
+    get_reg σ r2 = Some a ->
+    get_memory σ a = Some w ->
+    (ldr σ r1 r2) = (ExecI, (update_incr_PC (update_reg σ r1 w))).
   Proof.
-    intros.
+    intros ? ? ? ? Hneq Hcheck Hreg Hmem.
     unfold ldr.
     destruct r1 eqn:Heqn1,r2 eqn:Heqn2 ;try contradiction.
-    unfold bind.
-    simpl.
-    rewrite H4 H5.
-    destruct (get_mail_boxes σ1 !!! get_current_vm σ1).
-    simpl in H3.
-    destruct (decide (to_pid_aligned a = p)).
-    done.
-    done.
-  Qed.
-
-  Lemma ldr_FailPageFaultI_ldr_from_tx σ1 r1 r2 a :
-   PC ≠ r1 -> NZ ≠ r1 ->
-   PC ≠ r2 -> NZ ≠ r2 ->
-   (get_mail_boxes σ1 !!! get_current_vm σ1).1 = (to_pid_aligned a) ->
-   (get_reg σ1 r2) = Some a ->
-   (ldr σ1 r1 r2)= (FailPageFaultI, σ1).
-  Proof.
-    intros.
-    unfold ldr.
-    destruct r1 eqn:Heqn1,r2 eqn:Heqn2 ;try contradiction.
-    rewrite H4.
-    destruct (get_mail_boxes σ1 !!! get_current_vm σ1).
-    simpl in H3.
-    destruct (decide (to_pid_aligned a = p)).
-    done.
-    done.
-  Qed.
-
- Lemma ldr_FailPageFaultI_ldr_from_page σ1 r1 r2 a :
-   PC ≠ r1 -> NZ ≠ r1 ->
-   PC ≠ r2 -> NZ ≠ r2 ->
-   check_access_page σ1 (get_current_vm σ1) (tpa a) = false->
-   (get_reg σ1 r2) = Some a ->
-   (ldr σ1 r1 r2)= (FailPageFaultI, σ1).
-  Proof.
-    intros.
-    unfold ldr.
-    destruct r1 eqn:Heqn1,r2 eqn:Heqn2 ;try contradiction.
-    rewrite H4.
-    destruct (get_mail_boxes σ1 !!! get_current_vm σ1).
-    simpl in H3.
-    destruct (decide (to_pid_aligned a = p)).
-    done.
-    rewrite /get_memory /check_access_addr H3.
-    done.
-  Qed.
-
-  Lemma str_ExecI σ1 r1 r2 w a:
-   PC ≠ r1 -> NZ ≠ r1 ->
-   PC ≠ r2 -> NZ ≠ r2 ->
-   (get_mail_boxes σ1 !!! get_current_vm σ1).2.1 ≠ (to_pid_aligned a) ->
-   (get_reg σ1 r1) = Some w ->
-   (get_reg σ1 r2) = Some a ->
-   check_access_addr σ1 (get_current_vm σ1) a = true ->
-   (str σ1 r1 r2)= (ExecI, (update_offset_PC (update_memory_unsafe σ1 a w) 1)).
-  Proof.
-    intros.
-    unfold str.
-    destruct r1 eqn:Heqn1,r2 eqn:Heqn2 ;try contradiction.
-    unfold bind.
-    simpl.
-    rewrite H4 H5.
-    destruct ((get_mail_boxes σ1 !!! get_current_vm σ1)).
-    destruct p.
-    simpl in H3.
-    destruct (decide(to_pid_aligned a = p)).
-    done.
-    rewrite /update_memory /update_incr_PC /update_memory H6.
-    done.
-  Qed.
-
-  Lemma str_FailPageFaultI_str_to_rx σ1 r1 r2 w a :
-   PC ≠ r1 -> NZ ≠ r1 ->
-   PC ≠ r2 -> NZ ≠ r2 ->
-   (get_mail_boxes σ1 !!! get_current_vm σ1).2.1 = (to_pid_aligned a) ->
-   (get_reg σ1 r1) = Some w ->
-   (get_reg σ1 r2) = Some a ->
-   (str σ1 r1 r2)= (FailPageFaultI, σ1).
-  Proof.
-    intros.
-    unfold str.
-    destruct r1 eqn:Heqn1,r2 eqn:Heqn2 ;try contradiction.
-    rewrite H4 H5.
-    destruct (get_mail_boxes σ1 !!! get_current_vm σ1).
-    simpl in H3.
-    unfold bind.
-    simpl.
-    destruct p.
-    destruct (decide (tpa a = p)).
-    done.
-    done.
-  Qed.
-
- Lemma str_FailPageFaultI_str_to_page σ1 r1 r2 w a :
-   PC ≠ r1 -> NZ ≠ r1 ->
-   PC ≠ r2 -> NZ ≠ r2 ->
-   check_access_page σ1 (get_current_vm σ1) (tpa a) = false->
-   (get_reg σ1 r1) = Some w ->
-   (get_reg σ1 r2) = Some a ->
-   (str σ1 r1 r2)= (FailPageFaultI, σ1).
-  Proof.
-    intros.
-    unfold str.
-    destruct r1 eqn:Heqn1,r2 eqn:Heqn2 ;try contradiction.
-    rewrite H4 H5.
-    destruct (get_mail_boxes σ1 !!! get_current_vm σ1).
-    simpl in H3.
     rewrite /bind /=.
-    destruct p.
-    destruct (decide (to_pid_aligned a = p)).
+    rewrite Hreg.
+    rewrite /read_memory /check_read_access_addr /check_read_access_page Hcheck andb_true_l /=.
+    case_bool_decide;last done.
+    rewrite /get_memory in Hmem.
+    rewrite Hmem //.
+  Qed.
+
+  Lemma ldr_FailPageFaultI_ldr_from_tx σ r1 r2 a :
+    PC ≠ r1 -> NZ ≠ r1 ->
+    PC ≠ r2 -> NZ ≠ r2 ->
+    (get_mail_box σ @ (get_current_vm σ)).1 = (tpa a) ->
+    get_reg σ r2 = Some a ->
+    (ldr σ r1 r2) = (FailPageFaultI, σ).
+  Proof.
+    intros ? ? ? ? Heq Hreg.
+    unfold ldr.
+    destruct r1 eqn:Heqn1,r2 eqn:Heqn2 ;try contradiction.
+    rewrite Hreg.
+    rewrite /read_memory /check_read_access_addr /check_read_access_page.
+    case_bool_decide;first done.
+    rewrite andb_false_r //.
+  Qed.
+
+  Lemma ldr_FailPageFaultI_ldr_from_page σ1 r1 r2 a :
+    PC ≠ r1 -> NZ ≠ r1 ->
+    PC ≠ r2 -> NZ ≠ r2 ->
+    check_access_page σ1 (get_current_vm σ1) (tpa a) = false->
+    get_reg σ1 r2 = Some a ->
+    (ldr σ1 r1 r2) = (FailPageFaultI, σ1).
+  Proof.
+    intros ? ? ? ? Hcheck Hreg.
+    unfold ldr.
+    destruct r1 eqn:Heqn1,r2 eqn:Heqn2 ;try contradiction.
+    rewrite Hreg.
+    rewrite /read_memory /check_read_access_addr /check_read_access_page Hcheck.
+    rewrite andb_false_l //.
+  Qed.
+
+  Lemma str_ExecI σ r1 r2 w a:
+    PC ≠ r1 -> NZ ≠ r1 ->
+    PC ≠ r2 -> NZ ≠ r2 ->
+    (get_mail_box σ @ (get_current_vm σ)).2.1 ≠ (tpa a) ->
+    check_access_page σ (get_current_vm σ) (tpa a) = true ->
+    get_reg σ r1 = Some w ->
+    get_reg σ r2 = Some a ->
+    (str σ r1 r2) = (ExecI, (update_offset_PC (update_memory σ a w) 1)).
+  Proof.
+    intros ? ? ? ? Hneq Hcheck Hreg1 Hreg2.
+    unfold str.
+    destruct r1 eqn:Heqn1,r2 eqn:Heqn2 ;try contradiction.
+    rewrite /bind /=.
+    rewrite Hreg1 Hreg2.
+    rewrite /write_memory /check_write_access_addr /check_write_access_page Hcheck.
+    rewrite andb_true_l.
+    case_bool_decide;last done.
     done.
-    rewrite /update_memory  /check_access_addr H3 //.
+  Qed.
+
+  Lemma str_FailPageFaultI_str_to_rx σ r1 r2 w a :
+    PC ≠ r1 -> NZ ≠ r1 ->
+    PC ≠ r2 -> NZ ≠ r2 ->
+    (get_mail_box σ @ (get_current_vm σ)).2.1 = (tpa a) ->
+    get_reg σ r1 = Some w ->
+    get_reg σ r2 = Some a ->
+    (str σ r1 r2) = (FailPageFaultI, σ).
+  Proof.
+    intros ? ? ? ? Heq Hreg1 Hreg2.
+    unfold str.
+    destruct r1 eqn:Heqn1,r2 eqn:Heqn2 ;try contradiction.
+    rewrite Hreg1 Hreg2.
+    rewrite /bind /=.
+    rewrite /write_memory /check_write_access_addr /check_write_access_page.
+    case_bool_decide;first done.
+    rewrite andb_false_r //.
+  Qed.
+
+  Lemma str_FailPageFaultI_str_to_page σ r1 r2 w a :
+    PC ≠ r1 -> NZ ≠ r1 ->
+    PC ≠ r2 -> NZ ≠ r2 ->
+    check_access_page σ (get_current_vm σ) (tpa a) = false ->
+    get_reg σ r1 = Some w ->
+    get_reg σ r2 = Some a ->
+    (str σ r1 r2) = (FailPageFaultI, σ).
+  Proof.
+    intros ? ? ? ? Hcheck Hreg1 Hreg2.
+    unfold str.
+    destruct r1 eqn:Heqn1,r2 eqn:Heqn2 ;try contradiction.
+    rewrite Hreg1 Hreg2.
+    rewrite /bind /=.
+    rewrite /write_memory /check_write_access_addr /check_write_access_page.
+    rewrite Hcheck andb_false_l //.
   Qed.
 
   Lemma cmp_word_ExecI σ1 r w1 w2:
-   PC ≠ r -> NZ ≠ r ->
-   (get_reg σ1 r) = Some w1 ->
-   (cmp_word σ1 r w2)= (ExecI, (update_incr_PC (update_reg σ1 NZ
-            (if (w1 <? w2)%f then W2 else if (w2 <? w1)%f then W0 else W1)))).
+    PC ≠ r -> NZ ≠ r ->
+    get_reg σ1 r = Some w1 ->
+    (cmp_word σ1 r w2) =
+      (ExecI, (update_incr_PC (update_reg σ1 NZ (if (w1 <? w2)%f then W2 else if (w2 <? w1)%f then W0 else W1)))).
   Proof.
     intros.
     unfold cmp_word .
@@ -515,21 +495,21 @@ Qed.
     simpl.
     destruct ((w1 <? w2)%f).
     rewrite <- (option_state_unpack_preserve_state_Some σ1
-             (update_incr_PC (update_reg σ1 NZ W2)));eauto.
+                 (update_incr_PC (update_reg σ1 NZ W2)));eauto.
     destruct (w2 <? w1)%f.
     rewrite <- (option_state_unpack_preserve_state_Some σ1
-             (update_incr_PC (update_reg σ1 NZ W0)));eauto.
+                 (update_incr_PC (update_reg σ1 NZ W0)));eauto.
     done.
   Qed.
 
 
-   Lemma cmp_reg_ExecI σ1 r1 w1 r2 w2:
-   PC ≠ r1 -> NZ ≠ r1 ->
-   PC ≠ r2 -> NZ ≠ r2 ->
-   (get_reg σ1 r1) = Some w1 ->
-   (get_reg σ1 r2) = Some w2 ->
-   (cmp_reg σ1 r1 r2)= (ExecI, (update_incr_PC (update_reg σ1 NZ
-            (if (w1 <? w2)%f then W2 else if (w2 <? w1)%f then W0 else W1)))).
+  Lemma cmp_reg_ExecI σ1 r1 w1 r2 w2:
+    PC ≠ r1 -> NZ ≠ r1 ->
+    PC ≠ r2 -> NZ ≠ r2 ->
+    get_reg σ1 r1 = Some w1 ->
+    get_reg σ1 r2 = Some w2 ->
+    (cmp_reg σ1 r1 r2) =
+      (ExecI, (update_incr_PC (update_reg σ1 NZ (if (w1 <? w2)%f then W2 else if (w2 <? w1)%f then W0 else W1)))).
   Proof.
     intros.
     unfold cmp_reg.
@@ -539,64 +519,60 @@ Qed.
     simpl.
     destruct ((w1 <? w2)%f).
     rewrite <- (option_state_unpack_preserve_state_Some σ1
-             (update_incr_PC (update_reg σ1 NZ W2)));eauto.
+                                                        (update_incr_PC (update_reg σ1 NZ W2)));eauto.
     destruct (w2 <? w1)%f.
     rewrite <- (option_state_unpack_preserve_state_Some σ1
-             (update_incr_PC (update_reg σ1 NZ W0)));eauto.
+                                                        (update_incr_PC (update_reg σ1 NZ W0)));eauto.
     done.
   Qed.
 
   Lemma add_ExecI σ1 r1 w1 r2 w2:
-   PC ≠ r1 -> NZ ≠ r1 ->
-   PC ≠ r2 -> NZ ≠ r2 ->
-   (get_reg σ1 r1) = Some w1 ->
-   (get_reg σ1 r2) = Some w2 ->
-   (add σ1 r1 r2)= (ExecI, (update_incr_PC (update_reg σ1 r1 (w1 ^+ (finz.to_z w2))%f))).
+    PC ≠ r1 -> NZ ≠ r1 ->
+    PC ≠ r2 -> NZ ≠ r2 ->
+    get_reg σ1 r1 = Some w1 ->
+    get_reg σ1 r2 = Some w2 ->
+    (add σ1 r1 r2) = (ExecI, (update_incr_PC (update_reg σ1 r1 (w1 ^+ (finz.to_z w2))%f))).
   Proof.
     intros.
     unfold add.
-    (* destruct r1;[contradiction|contradiction|]. *)
-    (* destruct r2; [contradiction|contradiction|]. *)
-    (* TODO: add validity check of regs in opsem *)
+    destruct r1;[contradiction|contradiction|].
+    destruct r2; [contradiction|contradiction|].
     rewrite H3 H4.
     done.
   Qed.
 
   Lemma sub_ExecI σ1 r1 w1 r2 w2:
-   PC ≠ r1 -> NZ ≠ r1 ->
-   PC ≠ r2 -> NZ ≠ r2 ->
-   (get_reg σ1 r1) = Some w1 ->
-   (get_reg σ1 r2) = Some w2 ->
-   (sub σ1 r1 r2)= (ExecI, (update_incr_PC (update_reg σ1 r1 (w1 ^- (finz.to_z w2))%f))).
+    PC ≠ r1 -> NZ ≠ r1 ->
+    PC ≠ r2 -> NZ ≠ r2 ->
+    get_reg σ1 r1 = Some w1 ->
+    get_reg σ1 r2 = Some w2 ->
+    (sub σ1 r1 r2) = (ExecI, (update_incr_PC (update_reg σ1 r1 (w1 ^- (finz.to_z w2))%f))).
   Proof.
     intros.
     unfold sub.
-    (* destruct r1;[contradiction|contradiction|]. *)
-    (* destruct r2; [contradiction|contradiction|]. *)
-    (* TODO: add validity check of regs in opsem *)
+    destruct r1;[contradiction|contradiction|].
+    destruct r2; [contradiction|contradiction|].
     rewrite H3 H4.
     done.
   Qed.
 
   Lemma mult_word_ExecI σ1 r1 w1 w2:
-   PC ≠ r1 -> NZ ≠ r1 ->
-   (get_reg σ1 r1) = Some w1 ->
-   (lang.mult σ1 r1 w2)= (ExecI, (update_incr_PC (update_reg σ1 r1 (w1 ^* (finz.to_z w2))%f))).
+    PC ≠ r1 -> NZ ≠ r1 ->
+    get_reg σ1 r1 = Some w1 ->
+    (lang.mult σ1 r1 w2) = (ExecI, (update_incr_PC (update_reg σ1 r1 (w1 ^* (finz.to_z w2))%f))).
   Proof.
     intros.
     unfold lang.mult.
-    (* destruct r1;[contradiction|contradiction|]. *)
-    (* destruct r2; [contradiction|contradiction|]. *)
-    (* TODO: add validity check of regs in opsem *)
+    destruct r1;[contradiction|contradiction|].
     rewrite H1.
     done.
   Qed.
 
   Lemma bne_ExecI σ1 w1 r w2:
-   PC ≠ r -> NZ ≠ r ->
-   (get_reg σ1 r) = Some w2 ->
-   (get_reg σ1 NZ) = Some w1 ->
-   (bne σ1 r)= (ExecI, if (w1 =? W1)%f then (update_incr_PC σ1) else (update_reg σ1 PC w2)).
+    PC ≠ r -> NZ ≠ r ->
+    (get_reg σ1 r) = Some w2 ->
+    (get_reg σ1 NZ) = Some w1 ->
+    (bne σ1 r)= (ExecI, if (w1 =? W1)%f then (update_incr_PC σ1) else (update_reg σ1 PC w2)).
   Proof.
     intros.
     unfold bne .
@@ -607,9 +583,9 @@ Qed.
   Qed.
 
   Lemma br_ExecI σ1 r w1:
-   PC ≠ r -> NZ ≠ r ->
-   (get_reg σ1 r) = Some w1 ->
-   (br σ1 r)= (ExecI,  (update_reg σ1 PC w1)).
+    PC ≠ r -> NZ ≠ r ->
+    (get_reg σ1 r) = Some w1 ->
+    (br σ1 r) = (ExecI, (update_reg σ1 PC w1)).
   Proof.
     intros.
     unfold br.
