theories/rules/rules_base.v
@@ -1,5 +1,5 @@
 From machine_program_logic.program_logic Require Import weakestpre.
-From HypVeri.algebra Require Import base reg pagetable mem.
+From HypVeri.algebra Require Import base reg pagetable mem mailbox.
 From HypVeri.lang Require Import lang_extra reg_extra.
 Require Import stdpp.fin.
 
@@ -47,13 +47,12 @@ Proof.
   rewrite /scheduled /machine.scheduler //= /scheduler.
 Qed.
 
-Lemma update_memory_unsafe_preserve_just_scheduled_vms {σ σ' n} a w:
-  just_scheduled_vms n σ (update_memory_unsafe σ' a w) = just_scheduled_vms n σ σ'.
+Lemma update_memory_preserve_just_scheduled_vms {σ σ' n} a w:
+  just_scheduled_vms n σ (update_memory σ' a w) = just_scheduled_vms n σ σ'.
 Proof.
   unfold just_scheduled_vms, just_scheduled.
   rewrite /scheduled /machine.scheduler //= /scheduler.
 Qed.
-
 
 Lemma scheduled_true {σ: state} i:
   get_current_vm σ = i ->  (scheduled σ i) = true.
@@ -79,13 +78,13 @@ Proof.
   rewrite /scheduled /machine.scheduler //= /scheduler.
 Qed.
 
-Lemma update_memory_unsafe_preserve_scheduled {σ} a w:
-  scheduled (update_memory_unsafe σ a w) = scheduled σ.
+Lemma update_memory_preserve_scheduled {σ} a w:
+  scheduled (update_memory σ a w) = scheduled σ.
 Proof.
   rewrite /scheduled /machine.scheduler //= /scheduler.
 Qed.
 
-Lemma not_valid_pc {s} i a :
+Lemma invalid_pc_not_accessible {s} i a :
   (tpa a) ∉ s ->
   {SS{{ ▷ (PC @@ i ->r a) ∗ ▷ i -@A> s }}}
   ExecI @ i
@@ -107,14 +106,15 @@ Proof.
   - iPureIntro.
     rewrite /reducible.
     exists FailI, σ1.
-    apply step_exec_fail_invalid_pc.
-    rewrite /is_valid_PC Hpc Hcur /=.
-    rewrite check_access_page_mem_eq in Hnacc.
-    rewrite Hnacc //.
+    eapply step_exec_fail_invalid_pc.
+    exact Hpc.
+    rewrite /read_memory /check_read_access_addr /check_read_access_page.
+    rewrite Hcur Hnacc.
+    rewrite andb_false_l //.
   - iModIntro.
     iIntros (m2 σ2) "? %HstepP".
     iModIntro.
-    inversion HstepP; subst.
+    inversion HstepP; simplify_eq.
     + simpl.
       rewrite /gen_vm_interp.
       iFrame.
@@ -124,33 +124,20 @@ Proof.
       iApply "Hϕ".
       iFrame.
     + simplify_eq.
-      rewrite /is_valid_PC Hpc in H.      
-      simpl in H.
-      rewrite check_access_page_mem_eq in Hnacc.
-      rewrite Hnacc in H.
-      inversion H.
+      rewrite /read_memory /check_read_access_addr /check_read_access_page in H0.
+      rewrite Hnacc andb_false_l // in H0.
     + simplify_eq.
-      rewrite /is_valid_PC Hpc in H.
-      simpl in H.
-      rewrite check_access_page_mem_eq in Hnacc.
-      rewrite Hnacc in H.
-      inversion H.
+      rewrite /read_memory /check_read_access_addr /check_read_access_page in H0.
+      rewrite Hnacc andb_false_l // in H0.
 Qed.
 
-Lemma not_valid_instr {q s} i a wi :
-  decode_instruction wi = None ->
-  (tpa a) ∈ s ->
-  {SS{{ ▷ (PC @@ i ->r a)
-        ∗ ▷ i -@{q}A> s
-        ∗ ▷ a ->a wi}}}
+Lemma invalid_pc_in_tx {p_tx} i a :
+  (tpa a) = p_tx ->
+  {SS{{ ▷ (PC @@ i ->r a) ∗ ▷ TX@i := p_tx }}}
   ExecI @ i
-  {{{ RET (false, FailI);
-    PC @@ i ->r a
-    ∗ i -@{q}A> s
-    ∗ a ->a wi
-  }}}.
+  {{{ RET (false, FailI); PC @@ i ->r a ∗ TX@i := p_tx}}}.
 Proof.
-  iIntros (Hdecode_none Hin ϕ) "(>Hpc & >Ha & >Hw) Hϕ".
+  iIntros (Hmm ϕ) "(>Hpc & >Htx) Hϕ".
   iApply (sswp_lift_atomic_step ExecI);[done|].
   iIntros (n σ1) "%Hsche Hσ1".
   rewrite /scheduled /= /scheduler /Is_true in Hsche.
@@ -159,29 +146,89 @@ Proof.
   apply fin_to_nat_inj in Heqb.
   rename Heqb into Hcur.
   iModIntro.
-  iDestruct "Hσ1" as "( ? & Hmem & Hreg & ? & ? & ? & Haccess & ?)".
+  iDestruct "Hσ1" as "( ? & ? & Hreg & Hmb & ? & ? & Haccess & ?)".
   iDestruct (gen_reg_valid1 PC i a Hcur with "Hreg Hpc") as "%Hpc".
-  iDestruct (access_agree_check_true (tpa a) i with "Haccess Ha") as "%Hacc";first auto.
-  iDestruct (gen_mem_valid with "Hmem Hw") as "%Hlookup_w".
+  iDestruct (mb_valid_tx i p_tx with "Hmb Htx") as "%Heq_tx".
   iSplit.
   - iPureIntro.
     rewrite /reducible.
     exists FailI, σ1.
-    rewrite check_access_page_mem_eq in Hacc.
+    eapply step_exec_fail_invalid_pc.
+    exact Hpc.
+    rewrite /read_memory /check_read_access_addr /check_read_access_page.
+    rewrite Hcur Hmm.
+    case_bool_decide;first done.
+    rewrite andb_false_r //.
+  - iModIntro.
+    iIntros (m2 σ2) "? %HstepP".
+    iModIntro.
+    inversion HstepP; simplify_eq.
+    + simpl.
+      rewrite /gen_vm_interp.
+      iFrame.
+      rewrite just_scheduled_vms_no_step_empty.
+      iSplitR;[done|].
+      rewrite andb_false_intro2;auto.
+      iApply "Hϕ".
+      iFrame.
+    + simplify_eq.
+      rewrite /read_memory /check_read_access_addr /check_read_access_page in H0.
+      case_bool_decide;first done.
+      rewrite andb_false_r // in H0.
+    + simplify_eq.
+      rewrite /read_memory /check_read_access_addr /check_read_access_page in H0.
+      case_bool_decide;first done.
+      rewrite andb_false_r // in H0.
+Qed.
+
+
+Lemma not_valid_instr {q s p_tx} i a wi :
+  decode_instruction wi = None ->
+  (tpa a) ∈ s ->
+  (tpa a) ≠ p_tx ->
+  {SS{{ ▷ (PC @@ i ->r a)
+        ∗ ▷ i -@{q}A> s
+        ∗ ▷ TX@i := p_tx
+        ∗ ▷ a ->a wi}}}
+  ExecI @ i
+  {{{ RET (false, FailI);
+    PC @@ i ->r a
+    ∗ i -@{q}A> s
+    ∗ a ->a wi
+  }}}.
+Proof.
+  iIntros (Hdecode_none Hin Hneq ϕ) "(>Hpc & >Ha & >tx & >Hw) Hϕ".
+  iApply (sswp_lift_atomic_step ExecI);[done|].
+  iIntros (n σ1) "%Hsche Hσ1".
+  rewrite /scheduled /= /scheduler /Is_true in Hsche.
+  case_match;[|done].
+  apply bool_decide_eq_true in Heqb.
+  apply fin_to_nat_inj in Heqb.
+  rename Heqb into Hcur.
+  iModIntro.
+  iDestruct "Hσ1" as "( ? & Hmem & Hreg & Hmb & ? & ? & Haccess & ?)".
+  iDestruct (gen_reg_valid1 PC i a Hcur with "Hreg Hpc") as "%Hpc".
+  iDestruct (access_agree_check_true (tpa a) i with "Haccess Ha") as "%Hacc";first auto.
+  iDestruct (gen_mem_valid with "Hmem Hw") as "%Hlookup_w".
+  iDestruct (mb_valid_tx i p_tx with "Hmb tx") as "%Heq_tx".
+  iSplit.
+  - iPureIntro.
+    rewrite /reducible.
+    exists FailI, σ1.
     eapply step_exec_fail_invalid_instr;eauto.
-    rewrite /is_valid_PC Hpc Hcur /=.
-    rewrite Hacc //.
-    rewrite /get_memory Hcur Hacc //.
+    rewrite /read_memory /check_read_access_addr /check_read_access_page Hcur Hacc.
+    rewrite andb_true_l.
+    rewrite -Heq_tx in Hneq.
+    case_bool_decide; done.
   - iModIntro.
     iIntros (m2 σ2) "? %HstepP".
     iModIntro.
     inversion HstepP; subst.
     + simplify_eq.
-      rewrite /is_valid_PC Hpc in H.
-      simpl in H.
-      rewrite check_access_page_mem_eq in Hacc.
-      rewrite Hacc in H.
-      contradiction.
+      rewrite /read_memory /check_read_access_addr /check_read_access_page Hacc andb_true_l in H0.
+      case_bool_decide.
+      rewrite H0 // in Hlookup_w.
+      rewrite H // in Hneq.
     + simpl. rewrite /gen_vm_interp.
       iFrame.
       rewrite just_scheduled_vms_no_step_empty.
@@ -189,14 +236,14 @@ Proof.
       rewrite andb_false_intro2;auto.
       iApply "Hϕ".
       iFrame.
-    + rewrite /get_memory in H1.
-      case_match.
-      rewrite H0 in Hpc.
-      inversion Hpc;subst.
-      rewrite Hlookup_w in H1.
-      inversion H1;subst w.
-      rewrite H2 // in Hdecode_none.
-      rewrite check_access_page_mem_eq // in Hacc.
+    + simplify_eq.
+      rewrite /read_memory /check_read_access_addr /check_read_access_page Hacc andb_true_l in H0.
+      case_bool_decide.
+      rewrite H0 in Hlookup_w.
+      inversion Hlookup_w.
+      subst w.
+      rewrite H1 //in Hdecode_none.
+      rewrite H // in Hneq.
 Qed.
 
 End rules_base.
